examples/mw/MWMap01proof.v
@@ -1,0 +1,530 @@
+Require Import MWMap0 MWMap1 HoareDef SimModSem.
+Require Import Coqlib.
+Require Import ImpPrelude.
+Require Import Skeleton.
+Require Import PCM.
+Require Import ModSem Behavior.
+Require Import Relation_Definitions.
+
+(*** TODO: export these in Coqlib or Universe ***)
+Require Import Relation_Operators.
+Require Import RelationPairs.
+From ITree Require Import
+     Events.MapDefault.
+From ExtLib Require Import
+     Core.RelDec
+     Structures.Maps
+     Data.Map.FMapAList.
+Require Import HTactics ProofMode IPM.
+Require Import MWHeader Mem1 STB.
+
+Set Implicit Arguments.
+
+Local Open Scope nat_scope.
+
+
+
+
+Section SIMMODSEM.
+
+  Context `{Σ: GRA.t}.
+  Context `{@GRA.inG memRA Σ}.
+  Context `{@GRA.inG mapRA Σ}.
+
+  Let W: Type := Any.t * Any.t.
+
+  Definition transl2 (hkvs: gmap mblock (list (Z * Z))): _mapRA :=
+    fun h =>
+      match hkvs !! h with
+      | Some kvs => Some (fun k => alist_find k kvs)
+      | _ => ε
+      end
+  .
+
+  (* Definition transl (hkvs: list (mblock * (list (Z * Z)))): _mapRA := *)
+  (*   fun h => *)
+  (*     match alist_find h hkvs with *)
+  (*     | Some kvs => Some (fun k => alist_find k kvs) *)
+  (*     | _ => ε *)
+  (*     end *)
+  (* . *)
+
+(*   Definition transl (hkvs: list (mblock * (list (Z * Z)))): _mapRA. *)
+(*     intros h. cbn. *)
+(*     destruct (alist_find h hkvs) eqn:T. *)
+(*     - apply Excl.just. intro k. *)
+(*       destruct (alist_find k l) eqn:U. *)
+(*       + apply (Some z). *)
+(*       + apply None. *)
+(*     - apply Excl.unit. *)
+(*   Defined. *)
+(* transl =  *)
+(* λ (hkvs : list (nat * list (Z * Z))) (h : nat), *)
+(*   let o := alist_find h hkvs in *)
+(*   let T : alist_find h hkvs = o := eq_refl in *)
+(*   match o as o0 return (alist_find h hkvs = o0 → Excl.car) with *)
+(*   | Some l => *)
+(*       λ _ : alist_find h hkvs = Some l, *)
+(*         Excl.just *)
+(*           (λ k : Z, *)
+(*              let o0 := alist_find k l in *)
+(*              let U : alist_find k l = o0 := eq_refl in *)
+(*              match o0 as o1 return (alist_find k l = o1 → option Z) with *)
+(*              | Some z => λ _ : alist_find k l = Some z, Some z *)
+(*              | None => λ _ : alist_find k l = None, None *)
+(*              end U) *)
+(*   | None => λ _ : alist_find h hkvs = None, Excl.unit *)
+(*   end T *)
+
+  Let wf: _ -> W -> Prop :=
+    @mk_wf _ unit
+           (fun _ _ _ =>
+              (∃ hkvs, ([∗ map] h ↦ kvs ∈ hkvs, ∃ hd, OwnM ((h,0%Z) |-> [hd]) ** is_map_internal hd kvs)
+                         ** OwnM (Auth.black (transl2 hkvs)))%I)
+  .
+  (* True **  *)
+  (* Inductive sim_loc: URA.car (t:=(Excl.t _)) -> option (list val) -> option (list val) -> Prop := *)
+  (* | sim_loc_k stk0: sim_loc (Some stk0) None (Some stk0) *)
+  (* | sim_loc_u stk0: sim_loc ε (Some stk0) (Some stk0) *)
+  (* | sim_loc_absent: sim_loc ε None None *)
+  (* . *)
+
+  (* Notation sim res0 mgr_src0 mgr_tgt0 := *)
+  (*   (∀ h, sim_loc ((res0: URA.car (t:=_stkRA)) h) *)
+  (*                 ((mgr_src0: gmap mblock (list val)) !! h) ((mgr_tgt0: gmap mblock (list val)) !! h)). *)
+
+  (* Let wf: _ -> W -> Prop := *)
+  (*   @mk_wf _ unit *)
+  (*          (fun _ _mgr_src0 _mgr_tgt0 => *)
+  (*             (∃ mgr_src0 mgr_tgt0 (res0: URA.car (t:=_stkRA)), *)
+  (*                 (⌜(<<SRC: _mgr_src0 = mgr_src0↑>>) /\ (<<TGT: _mgr_tgt0 = mgr_tgt0↑>>) /\ *)
+  (*                  (<<SIM: sim res0 mgr_src0 mgr_tgt0>>)⌝) *)
+  (*                 ∧ ({{"O": OwnM ((Auth.black res0): URA.car (t:=stkRA))}}) *)
+  (*             )%I) *)
+  (* . *)
+
+
+
+  (* From iris.algebra Require Import big_op. *)
+  (* From iris.bi Require Import big_op. *)
+
+  (* Let wf: _ -> W -> Prop := *)
+  (*   @mk_wf _ unit *)
+  (*          (fun _ _stk_mgr0 _ => *)
+  (*             ⌜True⌝ ** (∃ (stk_mgr0: gmap mblock (list val)), *)
+  (*                        (⌜_stk_mgr0 = stk_mgr0↑⌝) ∧ *)
+  (*                        ({{"SIM": ([∗ map] handle ↦ stk ∈ stk_mgr0, *)
+  (*                                   (∃ hd, OwnM ((handle, 0%Z) |-> [hd]) ** is_list hd stk))}}) *)
+  (*          )) *)
+  (* . *)
+
+  Variable global_stb: Sk.t -> gname -> option fspec.
+  Hypothesis STBINCL: forall sk, stb_incl (to_stb (MapStb ++ MemStb)) (global_stb sk).
+
+  (* Ltac renamer := *)
+  (*   match goal with *)
+  (*   | [mp_src: gmap nat (list val) |- _ ] => *)
+  (*     let tmp := fresh "_tmp_" in *)
+  (*     rename mp_src into tmp; *)
+  (*     let name := fresh "stk_mgr0" in *)
+  (*     rename tmp into name *)
+  (*   end; *)
+  (*   match goal with *)
+  (*   | [ACC: current_iPropL _ ?Hns |- _ ] => *)
+  (*     match Hns with *)
+  (*     | context[(?name, ([∗ map] _↦_ ∈ _, _))%I] => mRename name into "SIM" *)
+  (*     end *)
+  (*   end *)
+  (* . *)
+
+  (* Ltac acatch := *)
+  (*   match goal with *)
+  (*   | [ |- (gpaco8 (_sim_itree _ _) _ _ _ _ _ _ _ _ _ (_, _) (_, trigger (Call ?fn ?args) >>= _)) ] => *)
+  (*     astep fn (tt↑) *)
+  (*   end. *)
+  Theorem correct: refines2 [MWMap0.Map] [MWMap1.Map global_stb].
+  Proof.
+    eapply adequacy_local2. econs; ss.
+    i. econstructor 1 with (wf:=wf) (le:=top2); et; swap 2 3.
+    { typeclasses eauto. }
+    { esplits; et. ss. econs; et. eapply to_semantic. iIntros "H". iExists ∅. iFrame. iSplitL; ss. }
+
+    econs; ss.
+    { init. harg. mDesAll; des; clarify. fold wf.
+      unfold newF, ccallU. steps. astart 2.
+      acatch.
+      { eapply STBINCL. stb_tac; ss. }
+      hcall _ (1) _ with "*".
+      { iModIntro.
+        (*** TODO: iSplits; ss; et gives weird goal ***)
+        (* Global Opaque Pure And Sepconj Own OwnM Ex. *)
+        iSplitL; [|iSplits; ss; et]; cycle 1.
+        iExists _. iFrame. }
+      { esplits; ss; et. eapply OrdArith.lt_from_nat; lia. }
+      fold wf. mDesAll; des; clarify. steps. force_r; ss. steps.
+      acatch.
+      { eapply STBINCL. stb_tac; ss. }
+      hcall _ (_, _, _) _ with "*".
+      { iModIntro. iSplitL "INV1 A".
+        { iExists _. iFrame. }
+        iSplits; ss; et.
+      }
+      { esplits; ss; et. eapply OrdArith.lt_from_nat; lia. }
+      fold wf. mDesAll; des; clarify. steps. astop. steps. force_l. esplits. steps.
+      rename a4 into hkvs. rename a2 into h.
+      mAssertPure (hkvs !! h = None).
+      { destruct (hkvs !! h) eqn:T; ss.
+        (* Search big_opM. *)
+        iDestruct (big_sepM_lookup with "INV") as "B"; et. iDes.
+        iExFalso. iApply (points_to_disj with "B"); eauto.
+      }
+      mAssert ([∗ map] h↦kvs ∈ <[h:=[]]>hkvs, ∃ hd, OwnM((h,0%Z) |-> [hd]) ** is_map_internal hd kvs)%I
+        with "POST INV".
+      { iApply big_sepM_insert; ss. iFrame. ss. iSplits; ss; et. }
+      mAssert (#=> (OwnM (Auth.black (transl2 (<[h:=[]]>hkvs))) ** OwnM (is_map h (λ _, None)))) with "A".
+      { iPoseProof (OwnM_Upd with "A") as "A"; cycle 1.
+        { iMod "A". iModIntro. instantiate (1:=_ ⋅ _). iDestruct "A" as "[A B]". iFrame. }
+        rewrite URA.add_comm. unfold is_map.
+        etrans.
+        { eapply Auth.auth_alloc2. instantiate (1:=(_is_map h (λ _, None))).
+          mOwnWf "A". eapply Auth.black_wf in WF0. des.
+          clear - PURE WF0.
+          ur. i. ur in WF0. specialize (WF0 k).
+          destruct (dec k h).
+          - subst. clear WF0. unfold transl2, _is_map. ur. des_ifs. unfold alist in *. congruence.
+          - unfold _is_map. des_ifs. rewrite URA.unit_id. ss.
+        }
+        eapply URA.updatable_add; try refl.
+        clear - PURE.
+        erewrite f_equal; try refl. f_equal.
+        ur. unfold transl2, _is_map. extensionality h0.
+        destruct (dec h h0); subst.
+        - des_ifs_safe. unfold alist. rewrite PURE. rewrite URA.unit_idl. rewrite lookup_insert. ss.
+        - des_ifs_safe. unfold alist. rewrite URA.unit_id. rewrite lookup_insert_ne; ss.
+      }
+      mUpd "A2".
+      hret _; ss.
+      { iModIntro. iDestruct "A2" as "[A B]". iSplitL "A A1".
+        - iExists _. iFrame.
+        - iSplits; ss; et.
+      }
+    }
+
+    econs; ss.
+    { init. harg. mDesAll; des; clarify. fold wf.
+      des_ifs_safe; ss. mDesAll; des; clarify.
+      unfold updateF, ccallU. steps. astart 6.
+      rename n into nn.
+
+      acatch.
+      { eapply STBINCL. stb_tac; ss. }
+      hcall _ (3) _ with "A INV".
+      { iModIntro.
+        (*** TODO: iSplits; ss; et gives weird goal ***)
+        iSplitL; [|iSplits; ss; et]; cycle 1.
+        iExists _. iFrame. }
+      { esplits; ss; et. eapply OrdArith.lt_from_nat; lia. }
+      fold wf. mDesAll; des; clarify. steps.
+
+      rewrite points_to_split in *. rewrite Z.add_0_l in *. erewrite points_to_split with (ofs:=1%Z) in *.
+      mAssert _ with "A2".
+      { iDestruct "A2" as "[A [B C]]".
+        instantiate (1:=OwnM ((a2, 0%Z) |-> [Vundef]) ** OwnM ((a2, 1%Z) |-> [Vundef]) **
+                             OwnM ((a2, 2%Z) |-> [Vundef])). iFrame. }
+      mDesAll.
+
+      acatch.
+      { eapply STBINCL. stb_tac; ss. }
+      hcall _ (_, _, _) _ with "*".
+      { iModIntro. iSplitL "INV1 A".
+        { iExists _. iFrame. }
+        iSplits; ss; et.
+      }
+      { esplits; ss; et. eapply OrdArith.lt_from_nat; lia. }
+      fold wf. mDesAll; des; clarify. steps. astop. steps. force_l. esplits. steps.
+      rename a4 into hkvs. rename a2 into h.
+      mAssertPure (hkvs !! h = None).
+      { destruct (hkvs !! h) eqn:T; ss.
+        (* Search big_opM. *)
+        iDestruct (big_sepM_lookup with "INV") as "B"; et. iDes.
+        iExFalso. iApply (points_to_disj with "B"); eauto.
+      }
+      mAssert ([∗ map] h↦kvs ∈ <[h:=[]]>hkvs, ∃ hd, OwnM((h,0%Z) |-> [hd]) ** is_map_internal hd kvs)%I
+        with "POST INV".
+      { iApply big_sepM_insert; ss. iFrame. ss. iSplits; ss; et. }
+      mAssert (#=> (OwnM (Auth.black (transl2 (<[h:=[]]>hkvs))) ** OwnM (is_map h (λ _, None)))) with "A".
+      { iPoseProof (OwnM_Upd with "A") as "A"; cycle 1.
+        { iMod "A". iModIntro. instantiate (1:=_ ⋅ _). iDestruct "A" as "[A B]". iFrame. }
+        rewrite URA.add_comm. unfold is_map.
+        etrans.
+        { eapply Auth.auth_alloc2. instantiate (1:=(_is_map h (λ _, None))).
+          mOwnWf "A". eapply Auth.black_wf in WF0. des.
+          clear - PURE WF0.
+          ur. i. ur in WF0. specialize (WF0 k).
+          destruct (dec k h).
+          - subst. clear WF0. unfold transl2, _is_map. ur. des_ifs. unfold alist in *. congruence.
+          - unfold _is_map. des_ifs. rewrite URA.unit_id. ss.
+        }
+        eapply URA.updatable_add; try refl.
+        clear - PURE.
+        erewrite f_equal; try refl. f_equal.
+        ur. unfold transl2, _is_map. extensionality h0.
+        destruct (dec h h0); subst.
+        - des_ifs_safe. unfold alist. rewrite PURE. rewrite URA.unit_idl. rewrite lookup_insert. ss.
+        - des_ifs_safe. unfold alist. rewrite URA.unit_id. rewrite lookup_insert_ne; ss.
+      }
+      mUpd "A2".
+      hret _; ss.
+      { iModIntro. iDestruct "A2" as "[A B]". iSplitL "A A1".
+        - iExists _. iFrame.
+        - iSplits; ss; et.
+      }
+    }
+
+
+    -
+          Set Printing All.
+          unfold alist.
+          rewrite list_lookup_insert.
+          lookup_insert
+            lookup_insert_is_Some
+            lookup_insert_Some
+        admit "".
+        - refl.
+        rewrite add_disj_insert; ss.
+        { eapply (@pw_insert_wf); et.
+          { eapply Auth.black_wf; et. }
+          { ur; ss. }
+        }
+        specialize (WF1 h). destruct (res0 h) eqn:T; ss; et.
+        { spc SIM. rewrite T in *. inv SIM. rewrite _GUARANTEE in *. ss. }
+      }
+      { }
+      big_opM_insert_delete
+      big_sepM_insert_delete
+      big_opM_insert
+      big_sepM_insert
+      hret _; ss.
+            iFrame. iSplits; ss; et.
+        (*** TODO: iSplits; ss; et gives weird goal ***)
+        (* Global Opaque Pure And Sepconj Own OwnM Ex. *)
+        iSplitL; [|iSplits; ss; et]; cycle 1.
+        iExists _. iFrame. }
+        iSplits; ss; et. iFrame.
+      kinit. harg. fold wf. mDesAll; des; subst. ss.
+    }
+      
+      ss; et. iFrame. iLeft. iSplits; ss; et. }
+
+
+    econstructor 1 with (wf:=wf) (le:=top2); ss; et; swap 2 3.
+    { esplits. econs; ss. eapply to_semantic. iIntros "H". iClear "H". iSplits; ss. }
+  Qed.
+
+  Theorem sim_modsem: ModSemPair.sim (MWMap1.MapSem global_stb) MWMap0.MapSem.
+  Proof.
+    econstructor 1 with (wf:=wf) (le:=top2); ss; et; swap 2 3.
+    { esplits. econs; ss. eapply to_semantic. iIntros "H". iClear "H". iSplits; ss. }
+    econs; ss.
+    { unfold newF. kinit. harg. fold wf. mDesAll; des; subst. ss.
+      unfold new_body. steps. unfold ccallN, ccallU, cfunN, cfunU. steps.
+
+      astart 2. acatch. { eapply STBINCL. stb_tac; ss. } hcall _ (Some _) _ with "SIM"; ss; et.
+      { iModIntro. iSplits; ss; et.
+        { instantiate (1:=1%nat). ss. }
+        { iPureIntro. unfold_modrange_64. ss. }
+      }
+      { ss. }
+      Ltac post_call :=
+        fold wf; clear_fast; mDesAll; des_safe; subst; try rewrite Any.upcast_downcast in *; clarify; renamer.
+      post_call. rename a0 into handle.
+      steps.
+      force_r.
+      { ss. }
+      steps.
+
+      acatch. { eapply STBINCL. stb_tac; ss. } hcall _ (Some (_, _, _)) _ with "SIM A"; ss; et.
+      { iModIntro. iSplitL "SIM"; ss.
+        { iSplits; ss; et. }
+        { iSplits; ss; et. }
+      }
+      { ss. }
+      post_call. steps.
+      astop. steps.
+
+      force_l. exists handle. steps.
+      destruct (stk_mgr0 !! handle) eqn:T.
+      { mAssertPure False; ss.
+        (*** IEXPLOIT*) iDestruct (big_sepM_lookup_acc with "SIM") as "[B C]"; et. iDestruct "B" as (x) "[B D]".
+        iApply (points_to_disj with "POST B"); et.
+      }
+      astop. steps. astop. steps. force_l; ss. steps. astop. steps.
+
+      hret _; ss.
+      { iModIntro. iSplits; ss; et. iApply big_sepM_insert; ss. iFrame; ss; et. }
+      (*** ISPECIALIZE SYNTAX: iSpecialize ("A" $! _ _ H0). et. *)
+    }
+    econs; ss.
+    { unfold popF. kinit. harg. fold wf. mDesAll; des; subst. ss.
+      unfold pop_body, ccallU, cfunU.
+      steps. astop. steps. astop. steps. astop. steps. astart 7.
+
+      hide_k. destruct v; ss. des_ifs. clear_fast.
+      renamer. rename n into handle. rename l into stk. rename _UNWRAPU into T.
+      mAssert _ with "SIM".
+      { iDestruct (big_sepM_delete with "SIM") as "[B C]"; et. (* big_sepM_lookup_acc *)
+        instantiate (1:=_ ** _). iSplitL "B". { iExact "B". } iExact "C". }
+      mDesAll; ss. rename a into hd. renamer.
+
+      acatch. { eapply STBINCL. stb_tac; ss. } hcall _ (Some (_, _, _)) _ with "SIM A"; ss; et.
+      { iModIntro. iSplitL "SIM"; ss; et. }
+      { ss. }
+      post_call. unhide_k. steps.
+      hide_k.
+
+      force_r.
+      { mAssertPure _.
+        { iClear "SIM". iClear "POST". iApply is_list_wf. iApply "A2". }
+        des; clarify; et. des_ifs.
+      }
+      steps.
+
+      destruct stk as [|x stk1]; ss.
+      - mDesAll. subst.
+        unhide_k. steps. hide_k.
+        acatch. { eapply STBINCL. stb_tac; ss. } hcall (ord_pure 0) (Some (_, _)) _ with "SIM POST"; ss.
+        { iModIntro. iSplitL "SIM"; ss; [et|]. iSplits; ss. repeat iRight. et. }
+        post_call. unhide_k. steps. astop. steps.
+        force_r.
+        { ss. }
+        steps. astop. steps. astop. steps.
+
+        hret _; ss. iModIntro. iSplits; ss; et.
+        destruct (stk_mgr1 !! handle) eqn:U.
+        { iExFalso. iDestruct (big_sepM_lookup_acc with "SIM") as "[B C]"; et. iDestruct "B" as (x) "[SIM B]".
+          iApply (points_to_disj with "POST1 SIM"). }
+        iApply big_sepM_insert; ss. iSplitR "SIM"; et.
+      - mDesAll. subst. rename a into hd. rename a0 into tl. rewrite points_to_split in ACC. mDesOwn "A1".
+        rewrite Z.add_0_l in *.
+        unhide_k. steps. hide_k.
+
+        acatch. { eapply STBINCL. stb_tac; ss. } hcall (ord_pure 0) (Some (_, _)) _ with "SIM A1"; ss.
+        { iModIntro. iSplitL "SIM"; ss. { et. } iSplits; ss; et. }
+        post_call. unhide_k. steps.
+
+        force_r.
+        { ss. }
+        steps.
+
+        force_r.
+        { ss. }
+        steps.
+
+        unfold scale_int. uo. steps.
+        acatch. { eapply STBINCL. stb_tac; ss. } hcall (ord_pure 0) (Some (_, _, _)) _ with "SIM POST1"; ss.
+        { iModIntro. iSplitL "SIM"; ss; et. }
+        post_call. steps.
+
+        acatch. { eapply STBINCL. stb_tac; ss. } hcall (ord_pure 0) (Some (_, _, _)) _ with "SIM A2"; ss.
+        { iModIntro. iSplitL "SIM"; ss; et. }
+        post_call. steps.
+
+        acatch. { eapply STBINCL. stb_tac; ss. } hcall (ord_pure 0) (Some (_, _)) _ with "SIM POST2"; ss.
+        { iModIntro. iSplitL "SIM"; ss; et. }
+        post_call. steps.
+
+        acatch. { eapply STBINCL. stb_tac; ss. } hcall (ord_pure 0) (Some (_, _)) _ with "SIM POST1"; ss.
+        { iModIntro. iSplitL "SIM"; ss; et. }
+        post_call. steps.
+
+        acatch. { eapply STBINCL. stb_tac; ss. } hcall (ord_pure 0) (Some (_, _, _)) _ with "SIM POST"; ss.
+        { iModIntro. iSplitL "SIM"; ss; et. }
+        post_call. steps.
+
+        astop. steps. unfold pget. steps. renamer.
+
+        destruct (stk_mgr1 !! handle) eqn:V.
+        { mAssertPure False; ss. iDestruct (big_sepM_lookup_acc with "SIM") as "[B C]"; et.
+          iDestruct "B" as (y) "[SIM B]".
+          iApply (points_to_disj with "POST1 SIM"). }
+        steps. astop. steps. astop. steps.
+
+        hret _; ss.
+        { iModIntro. iSplits; ss; et. iApply big_sepM_insert; ss. iFrame. iExists _; ss. iFrame. }
+    }
+    econs; ss.
+    { unfold pushF. kinit. harg. fold wf. mDesAll; des; subst. ss.
+      unfold push_body, ccallU, cfunU.
+      steps. astop. steps. astop. steps. astop. steps. astart 7.
+
+      hide_k. destruct v; ss. des_ifs. clear_tac.
+      rename n into handle. renamer. rename l into stk. rename _UNWRAPU into T.
+      mAssert _ with "SIM".
+      { iDestruct (big_sepM_delete with "SIM") as "[B C]"; et. (* big_sepM_lookup_acc *)
+        instantiate (1:=_ ** _). iSplitL "B". { iExact "B". } iExact "C". }
+      mDesAll; ss. renamer. rename a into hd.
+
+      acatch. { eapply STBINCL. stb_tac; ss. } hcall (ord_pure 0) (Some _) _ with "SIM"; ss; et.
+      { iModIntro. iSplitL "SIM"; et. iSplits; ss; et.
+        { instantiate (1:=2). ss. }
+        { iPureIntro. ss. }
+      }
+      post_call. rename a0 into node. unhide_k. steps.
+
+      rewrite points_to_split in ACC. mDesOwn "A1". rewrite Z.add_0_l in *. clear_fast.
+
+      unfold scale_int. uo. steps.
+
+      force_r; ss. steps.
+
+      acatch. { eapply STBINCL. stb_tac; ss. } hcall (ord_pure 0) (Some (_, _, _)) _ with "A SIM"; ss; et.
+      { iModIntro. iSplitL "SIM"; et. }
+      post_call. steps.
+
+      acatch. { eapply STBINCL. stb_tac; ss. } hcall (ord_pure 0) (Some (_, _, _)) _ with "A1 SIM"; ss; et.
+      { iModIntro. iSplitL "SIM"; et. }
+      post_call. steps.
+
+      acatch. { eapply STBINCL. stb_tac; ss. } hcall (ord_pure 0) (Some (_, _, _)) _ with "A3 SIM"; ss; et.
+      { iModIntro. iSplitL "SIM"; et. }
+      post_call. steps.
+
+      acatch. { eapply STBINCL. stb_tac; ss. } hcall (ord_pure 0) (Some (_, _, _)) _ with "POST SIM"; ss; et.
+      { iModIntro. iSplitL "SIM"; et. }
+      post_call. steps.
+
+      astop. steps.
+
+      destruct (stk_mgr1 !! handle) eqn:V.
+      { mAssertPure False; ss. iDestruct (big_sepM_lookup_acc with "SIM") as "[B C]"; et.
+        iDestruct "B" as (y) "[SIM B]". iApply (points_to_disj with "POST3 SIM"). }
+
+      hret _; ss.
+      { iModIntro. iSplits; ss; et.
+        iApply big_sepM_insert; ss. iFrame. iExists _; ss. iFrame.
+        iExists _, _. iFrame. iSplit; ss. erewrite points_to_split with (hd:=v0) (tl:=[hd]).
+        iSplitL "POST1"; et.
+      }
+    }
+  Unshelve.
+    all: try exact 0. all: ss.
+  Qed.
+
+End SIMMODSEM.
+
+
+
+Section SIMMOD.
+
+  Context `{Σ: GRA.t}.
+  Context `{@GRA.inG memRA Σ}.
+
+  Variable global_stb: Sk.t -> gname -> option fspec.
+  Hypothesis STBINCL: forall sk, stb_incl (to_stb (StackStb ++ MemStb)) (global_stb sk).
+
+  Theorem correct: refines2 [Stack0.Stack] [Stack1.Stack global_stb].
+  Proof.
+    eapply adequacy_local2. econs; ss. ii. eapply sim_modsem; ss.
+  Qed.
+
+End SIMMOD.
